        $((p\vee q)\Rightarrow r)\Rightarrow p$

$\Leftrightarrow(\neg(p\vee q)\vee r)\Rightarrow p$   ，Using ($A\Rightarrow B\equiv \neg A \vee B$) here.

$\Leftrightarrow \neg(\neg (p\vee q)\vee r)\vee p$ ,    Using $(A\Rightarrow B\equiv \neg A \vee B)$ here.

$\Leftrightarrow ((p\vee q)\wedge \neg r)\vee p$,      Using ($\neg (A\wedge B)\equiv (\neg A \wedge \neg B)$) here.

$\Leftrightarrow (p\vee q)\wedge (\neg r \vee p)$  ,     Using  $(A\wedge B)\vee C \equiv (A\vee C)\wedge (B\vee C)$ 

$\Leftrightarrow (p\wedge \neg r)\vee (q\wedge \neg r)\vee p$,     Using $ (A\vee B)\wedge C \equiv (A\wedge C)\vee (B\wedge C)$







Let $a,b\in \mathbb{R}$, prove that $\left| a+b\right|^{n}\leq 2^{n-1}(\left|a\right|^{n}+\left|b\right|^{n})$, $n\in \mathbb{N}$
